pheap as a data structure rather than a pair.

HOL/SepLogic/SepAuto.thy
@@ -7,7 +7,10 @@ begin
 
 section {* Partial Heaps *}
 
-type_synonym pheap = "heap \<times> addr set"
+datatype pheap = pHeap (heapOf: heap) (addrOf: "addr set")
+setup {* add_rewrite_rule_back_cond @{thm pheap.collapse} [with_cond "?pheap \<noteq> pHeap ?a ?b"] *}
+setup {* add_forward_prfstep (equiv_forward_th @{thm pheap.simps(1)}) *}
+setup {* fold add_rewrite_rule @{thms pheap.sel} *}
 
 fun in_range :: "(heap \<times> addr set) \<Rightarrow> bool" where
   "in_range (h,as) \<longleftrightarrow> (\<forall>a\<in>as. a < lim h)"
@@ -47,12 +50,16 @@ setup {* add_rewrite_rule @{thm aseval.simps} *}
 
 definition proper :: "assn_raw \<Rightarrow> bool" where [rewrite]:
   "proper P = (
-    (\<forall>h as. aseval P (h,as) \<longrightarrow> in_range (h,as)) \<and>
-    (\<forall>h h' as. aseval P (h,as) \<longrightarrow> relH as h h' \<longrightarrow> in_range (h',as) \<longrightarrow> aseval P (h',as)))"
+    (\<forall>h as. aseval P (pHeap h as) \<longrightarrow> in_range (h,as)) \<and>
+    (\<forall>h h' as. aseval P (pHeap h as) \<longrightarrow> relH as h h' \<longrightarrow> in_range (h',as) \<longrightarrow> aseval P (pHeap h' as)))"
 setup {* add_property_const @{term proper} *}
 
+fun in_range_assn :: "pheap \<Rightarrow> bool" where
+  "in_range_assn (pHeap h as) \<longleftrightarrow> (\<forall>a\<in>as. a < lim h)"
+setup {* add_rewrite_rule @{thm in_range_assn.simps} *}
+
 typedef assn = "Collect proper"
-@proof @have "Assn in_range \<in> Collect proper" @qed
+@proof @have "Assn in_range_assn \<in> Collect proper" @qed
 
 setup {* add_rewrite_rule @{thm Rep_assn_inject} *}
 setup {* register_wellform_data ("Abs_assn P", ["proper P"]) *}
@@ -66,35 +73,35 @@ lemma proper_Rep_assn [forward]: "proper (Rep_assn P)" using Rep_assn by auto
 definition models :: "pheap \<Rightarrow> assn \<Rightarrow> bool" (infix "\<Turnstile>" 50) where [rewrite_bidir]:
   "h \<Turnstile> P \<longleftrightarrow> aseval (Rep_assn P) h"
 
-lemma models_in_range [resolve]: "h \<Turnstile> P \<Longrightarrow> in_range h" by auto2
+lemma models_in_range [resolve]: "pHeap h as \<Turnstile> P \<Longrightarrow> in_range (h,as)" by auto2
 
-lemma mod_relH [forward]: "relH as h h' \<Longrightarrow> (h, as) \<Turnstile> P \<Longrightarrow> (h', as) \<Turnstile> P" by auto2
+lemma mod_relH [forward]: "relH as h h' \<Longrightarrow> pHeap h as \<Turnstile> P \<Longrightarrow> pHeap h' as \<Turnstile> P" by auto2
 
 instantiation assn :: one begin
 definition one_assn :: assn where [rewrite]:
-  "1 \<equiv> Abs_assn (Assn (\<lambda>h. snd h = {}))"
+  "1 \<equiv> Abs_assn (Assn (\<lambda>h. addrOf h = {}))"
 instance .. end
 
 abbreviation one_assn :: assn ("emp") where "one_assn \<equiv> 1"
 
-lemma one_assn_rule [rewrite]: "h \<Turnstile> emp \<longleftrightarrow> snd h = {}" by auto2
+lemma one_assn_rule [rewrite]: "h \<Turnstile> emp \<longleftrightarrow> addrOf h = {}" by auto2
 setup {* del_prfstep_thm @{thm one_assn_def} *}
 
 instantiation assn :: times begin
 definition times_assn where [rewrite]:
   "P * Q = Abs_assn (Assn (
-    \<lambda>(h, as). (\<exists>as1 as2. as = as1 \<union> as2 \<and> as1 \<inter> as2 = {} \<and>
-                   aseval (Rep_assn P) (h, as1) \<and> aseval (Rep_assn Q) (h, as2))))"
+    \<lambda>h. (\<exists>as1 as2. addrOf h = as1 \<union> as2 \<and> as1 \<inter> as2 = {} \<and>
+                   aseval (Rep_assn P) (pHeap (heapOf h) as1) \<and> aseval (Rep_assn Q) (pHeap (heapOf h) as2))))"
 instance .. end
 
 lemma mod_star_conv [rewrite]:
-  "(h, as) \<Turnstile> A * B \<longleftrightarrow> (\<exists>as1 as2. as = as1 \<union> as2 \<and> as1 \<inter> as2 = {} \<and> (h, as1) \<Turnstile> A \<and> (h, as2) \<Turnstile> B)" by auto2
+  "pHeap h as \<Turnstile> A * B \<longleftrightarrow> (\<exists>as1 as2. as = as1 \<union> as2 \<and> as1 \<inter> as2 = {} \<and> pHeap h as1 \<Turnstile> A \<and> pHeap h as2 \<Turnstile> B)" by auto2
 setup {* del_prfstep_thm @{thm times_assn_def} *}
 
 lemma aseval_ext [backward]: "\<forall>h. aseval P h = aseval P' h \<Longrightarrow> P = P'"
   apply (cases P) apply (cases P') by auto
 
-lemma assn_ext: "\<forall>h as. (h, as) \<Turnstile> P \<longleftrightarrow> (h, as) \<Turnstile> Q \<Longrightarrow> P = Q"
+lemma assn_ext: "\<forall>h as. pHeap h as \<Turnstile> P \<longleftrightarrow> pHeap h as \<Turnstile> Q \<Longrightarrow> P = Q"
 @proof @have "Rep_assn P = Rep_assn Q" @qed
 setup {* add_backward_prfstep_cond @{thm assn_ext} [with_filt (order_filter "P" "Q")] *}
 
@@ -102,20 +109,20 @@ setup {* del_prfstep_thm @{thm aseval_ext} *}
 
 lemma assn_one_left: "1 * P = (P::assn)"
 @proof
-  @have "\<forall>h as. (h, as) \<Turnstile> P \<longleftrightarrow> (h, as) \<Turnstile> 1 * P" @with
+  @have "\<forall>h as. pHeap h as \<Turnstile> P \<longleftrightarrow> pHeap h as \<Turnstile> 1 * P" @with
     @have "as = {} \<union> as"
   @end
 @qed
 
 lemma assn_times_comm: "P * Q = Q * (P::assn)"
 @proof
-  @have "\<forall>h as. (h, as) \<Turnstile> P * Q \<longleftrightarrow> (h, as) \<Turnstile> Q * P" @with
-    @case "(h, as) \<Turnstile> P * Q" @with
-      @obtain as1 as2 where "as = as1 \<union> as2" "as1 \<inter> as2 = {}" "(h, as1) \<Turnstile> P" "(h, as2) \<Turnstile> Q"
+  @have "\<forall>h as. pHeap h as \<Turnstile> P * Q \<longleftrightarrow> pHeap h as \<Turnstile> Q * P" @with
+    @case "pHeap h as \<Turnstile> P * Q" @with
+      @obtain as1 as2 where "as = as1 \<union> as2" "as1 \<inter> as2 = {}" "pHeap h as1 \<Turnstile> P" "pHeap h as2 \<Turnstile> Q"
       @have "as = as2 \<union> as1"
     @end
-    @case "(h, as) \<Turnstile> Q * P" @with
-      @obtain as1 as2 where "as = as1 \<union> as2" "as1 \<inter> as2 = {}" "(h, as1) \<Turnstile> Q" "(h, as2) \<Turnstile> P"
+    @case "pHeap h as \<Turnstile> Q * P" @with
+      @obtain as1 as2 where "as = as1 \<union> as2" "as1 \<inter> as2 = {}" "pHeap h as1 \<Turnstile> Q" "pHeap h as2 \<Turnstile> P"
       @have "as = as2 \<union> as1"
     @end
   @end
@@ -123,15 +130,15 @@ lemma assn_times_comm: "P * Q = Q * (P::assn)"
 
 lemma assn_times_assoc: "(P * Q) * R = P * (Q * (R::assn))"
 @proof
-  @have "\<forall>h as. (h, as) \<Turnstile> (P * Q) * R \<longleftrightarrow> (h, as) \<Turnstile> P * (Q * R)" @with
-    @case "(h, as) \<Turnstile> (P * Q) * R" @with
-      @obtain as1 as2 where "as = as1 \<union> as2" "as1 \<inter> as2 = {}" "(h, as1) \<Turnstile> P * Q" "(h, as2) \<Turnstile> R"
-      @obtain as11 as12 where "as1 = as11 \<union> as12" "as11 \<inter> as12 = {}" "(h, as11) \<Turnstile> P" "(h, as12) \<Turnstile> Q"
+  @have "\<forall>h as. pHeap h as \<Turnstile> (P * Q) * R \<longleftrightarrow> pHeap h as \<Turnstile> P * (Q * R)" @with
+    @case "pHeap h as \<Turnstile> (P * Q) * R" @with
+      @obtain as1 as2 where "as = as1 \<union> as2" "as1 \<inter> as2 = {}" "pHeap h as1 \<Turnstile> P * Q" "pHeap h as2 \<Turnstile> R"
+      @obtain as11 as12 where "as1 = as11 \<union> as12" "as11 \<inter> as12 = {}" "pHeap h as11 \<Turnstile> P" "pHeap h as12 \<Turnstile> Q"
       @have "as = as11 \<union> (as12 \<union> as2)"
     @end
-    @case "(h, as) \<Turnstile> P * (Q * R)" @with
-      @obtain as1 as2 where "as = as1 \<union> as2" "as1 \<inter> as2 = {}" "(h, as1) \<Turnstile> P" "(h, as2) \<Turnstile> Q * R"
-      @obtain as21 as22 where "as2 = as21 \<union> as22" "as21 \<inter> as22 = {}" "(h, as21) \<Turnstile> Q" "(h, as22) \<Turnstile> R"
+    @case "pHeap h as \<Turnstile> P * (Q * R)" @with
+      @obtain as1 as2 where "as = as1 \<union> as2" "as1 \<inter> as2 = {}" "pHeap h as1 \<Turnstile> P" "pHeap h as2 \<Turnstile> Q * R"
+      @obtain as21 as22 where "as2 = as21 \<union> as22" "as21 \<inter> as22 = {}" "pHeap h as21 \<Turnstile> Q" "pHeap h as22 \<Turnstile> R"
       @have "as = (as1 \<union> as21) \<union> as22"
     @end
   @end
@@ -152,11 +159,11 @@ setup {* del_prfstep_thm @{thm ex_assn_def} *}
 
 lemma ex_distrib_star: "(\<exists>\<^sub>Ax. P x * Q) = (\<exists>\<^sub>Ax. P x) * Q"
 @proof
-  @have "\<forall>h as. (h, as) \<Turnstile> (\<exists>\<^sub>Ax. P x) * Q \<longleftrightarrow> (h, as) \<Turnstile> (\<exists>\<^sub>Ax. P x * Q)" @with
-    @case "(h, as) \<Turnstile> (\<exists>\<^sub>Ax. P x) * Q" @with
-      @obtain as1 as2 where "as = as1 \<union> as2" "as1 \<inter> as2 = {}" "(h, as1) \<Turnstile> (\<exists>\<^sub>Ax. P x)" "(h, as2) \<Turnstile> Q"
-      @obtain x where "(h, as1) \<Turnstile> P x"
-      @have "(h, as) \<Turnstile> P x * Q"
+  @have "\<forall>h as. pHeap h as \<Turnstile> (\<exists>\<^sub>Ax. P x) * Q \<longleftrightarrow> pHeap h as \<Turnstile> (\<exists>\<^sub>Ax. P x * Q)" @with
+    @case "pHeap h as \<Turnstile> (\<exists>\<^sub>Ax. P x) * Q" @with
+      @obtain as1 as2 where "as = as1 \<union> as2" "as1 \<inter> as2 = {}" "pHeap h as1 \<Turnstile> (\<exists>\<^sub>Ax. P x)" "pHeap h as2 \<Turnstile> Q"
+      @obtain x where "pHeap h as1 \<Turnstile> P x"
+      @have "pHeap h as \<Turnstile> P x * Q"
     @end
   @end
 @qed
@@ -165,32 +172,32 @@ subsection {* Pointers *}
 
 definition sngr_assn :: "'a::heap ref \<Rightarrow> 'a \<Rightarrow> assn" (infix "\<mapsto>\<^sub>r" 82) where [rewrite]:
   "r \<mapsto>\<^sub>r x = Abs_assn (Assn (
-    \<lambda>(h, as). Ref.get h r = x \<and> as = {addr_of_ref r} \<and> addr_of_ref r < lim h))"
+    \<lambda>h. Ref.get (heapOf h) r = x \<and> addrOf h = {addr_of_ref r} \<and> addr_of_ref r < lim (heapOf h)))"
 
 lemma sngr_assn_rule [rewrite]:
-  "(h, as) \<Turnstile> r \<mapsto>\<^sub>r x \<longleftrightarrow> (Ref.get h r = x \<and> as = {addr_of_ref r} \<and> addr_of_ref r < lim h)" by auto2
+  "pHeap h as \<Turnstile> r \<mapsto>\<^sub>r x \<longleftrightarrow> (Ref.get h r = x \<and> as = {addr_of_ref r} \<and> addr_of_ref r < lim h)" by auto2
 setup {* del_prfstep_thm @{thm sngr_assn_def} *}
 
 definition snga_assn :: "'a::heap array \<Rightarrow> 'a list \<Rightarrow> assn" (infix "\<mapsto>\<^sub>a" 82) where [rewrite]:
   "r \<mapsto>\<^sub>a x = Abs_assn (Assn (
-    \<lambda>(h, as). Array.get h r = x \<and> as = {addr_of_array r} \<and> addr_of_array r < lim h))"
+    \<lambda>h. Array.get (heapOf h) r = x \<and> addrOf h = {addr_of_array r} \<and> addr_of_array r < lim (heapOf h)))"
 
 lemma snga_assn_rule [rewrite]:
-  "(h, as) \<Turnstile> r \<mapsto>\<^sub>a x \<longleftrightarrow> (Array.get h r = x \<and> as = {addr_of_array r} \<and> addr_of_array r < lim h)" by auto2
+  "pHeap h as \<Turnstile> r \<mapsto>\<^sub>a x \<longleftrightarrow> (Array.get h r = x \<and> as = {addr_of_array r} \<and> addr_of_array r < lim h)" by auto2
 setup {* del_prfstep_thm @{thm snga_assn_def} *}
 
 subsection {* Pure Assertions *}
 
 definition pure_assn :: "bool \<Rightarrow> assn" ("\<up>") where [rewrite]:
-  "\<up>b = Abs_assn (Assn (\<lambda>h. snd h = {} \<and> b))"
+  "\<up>b = Abs_assn (Assn (\<lambda>h. addrOf h = {} \<and> b))"
 
-lemma pure_assn_rule [rewrite]: "h \<Turnstile> \<up>b \<longleftrightarrow> (snd h = {} \<and> b)" by auto2
+lemma pure_assn_rule [rewrite]: "h \<Turnstile> \<up>b \<longleftrightarrow> (addrOf h = {} \<and> b)" by auto2
 setup {* del_prfstep_thm @{thm pure_assn_def} *}
 
 definition top_assn :: assn ("true") where [rewrite]:
-  "top_assn = Abs_assn (Assn in_range)"
+  "top_assn = Abs_assn (Assn in_range_assn)"
 
-lemma top_assn_rule [rewrite]: "h \<Turnstile> true \<longleftrightarrow> in_range h" by auto2
+lemma top_assn_rule [rewrite]: "pHeap h as \<Turnstile> true \<longleftrightarrow> in_range (h, as)" by auto2
 setup {* del_prfstep_thm @{thm top_assn_def} *}
 
 setup {* del_prfstep_thm @{thm models_def} *}
@@ -202,7 +209,7 @@ abbreviation bot_assn :: assn ("false") where "bot_assn \<equiv> \<up>False"
 lemma mod_false' [resolve]: "\<not> (h \<Turnstile> false * Ru)" by auto2
 
 lemma mod_star_trueI [backward]: "h \<Turnstile> P \<Longrightarrow> h \<Turnstile> P * true"
-@proof @have "snd h = snd h \<union> {}" @qed
+@proof @have "addrOf h = addrOf h \<union> {}" @qed
 
 lemma top_assn_reduce: "true * true = true" by auto2
 setup {* del_prfstep_thm @{thm mod_star_trueI} *}
@@ -211,7 +218,7 @@ lemma mod_pure_star_dist [rewrite]:
   "h \<Turnstile> P * \<up>b \<longleftrightarrow> (h \<Turnstile> P \<and> b)"
 @proof
   @case "h \<Turnstile> P \<and> b" @with
-    @have "snd h = snd h \<union> {}"
+    @have "addrOf h = addrOf h \<union> {}"
   @end
 @qed
 
@@ -286,8 +293,8 @@ definition new_addrs :: "heap \<Rightarrow> addr set \<Rightarrow> heap \<Righta
 lemma new_addr_refl [rewrite]: "new_addrs h as h = as" by auto2
 
 definition hoare_triple :: "assn \<Rightarrow> 'a Heap \<Rightarrow> ('a \<Rightarrow> assn) \<Rightarrow> bool" ("<_>/ _/ <_>") where [rewrite]:
-  "<P> c <Q> \<longleftrightarrow> (\<forall>h as \<sigma> r. (h, as) \<Turnstile> P \<longrightarrow> run c (Some h) \<sigma> r \<longrightarrow>
-    (\<sigma> \<noteq> None \<and> (the \<sigma>, new_addrs h as (the \<sigma>)) \<Turnstile> Q r \<and> relH {a . a < lim h \<and> a \<notin> as} h (the \<sigma>) \<and>
+  "<P> c <Q> \<longleftrightarrow> (\<forall>h as \<sigma> r. pHeap h as \<Turnstile> P \<longrightarrow> run c (Some h) \<sigma> r \<longrightarrow>
+    (\<sigma> \<noteq> None \<and> pHeap (the \<sigma>) (new_addrs h as (the \<sigma>)) \<Turnstile> Q r \<and> relH {a . a < lim h \<and> a \<notin> as} h (the \<sigma>) \<and>
      lim h \<le> lim (the \<sigma>)))"
 
 abbreviation hoare_triple' :: "assn \<Rightarrow> 'r Heap \<Rightarrow> ('r \<Rightarrow> assn) \<Rightarrow> bool" ("<_> _ <_>\<^sub>t") where
@@ -296,11 +303,11 @@ abbreviation hoare_triple' :: "assn \<Rightarrow> 'r Heap \<Rightarrow> ('r \<Ri
 lemma frame_rule [backward]:
   "<P> c <Q> \<Longrightarrow> <P * R> c <\<lambda>x. Q x * R>"
 @proof
-  @have "\<forall>h as \<sigma> r. (h, as) \<Turnstile> P * R \<longrightarrow> run c (Some h) \<sigma> r \<longrightarrow>
-                    (\<sigma> \<noteq> None \<and> (the \<sigma>, new_addrs h as (the \<sigma>)) \<Turnstile> Q r * R \<and>
+  @have "\<forall>h as \<sigma> r. pHeap h as \<Turnstile> P * R \<longrightarrow> run c (Some h) \<sigma> r \<longrightarrow>
+                    (\<sigma> \<noteq> None \<and> pHeap (the \<sigma>) (new_addrs h as (the \<sigma>)) \<Turnstile> Q r * R \<and>
                      relH {a . a < lim h \<and> a \<notin> as} h (the \<sigma>) \<and> lim h \<le> lim (the \<sigma>))" @with
-    @obtain as1 as2 where "as = as1 \<union> as2" "as1 \<inter> as2 = {}" "(h, as1) \<Turnstile> P \<and> (h, as2) \<Turnstile> R" @then
-    @have "relH as2 h (the \<sigma>)" @then
+    @obtain as1 as2 where "as = as1 \<union> as2" "as1 \<inter> as2 = {}" "pHeap h as1 \<Turnstile> P \<and> pHeap h as2 \<Turnstile> R"
+    @have "relH as2 h (the \<sigma>)"
     @have "new_addrs h as (the \<sigma>) = new_addrs h as1 (the \<sigma>) \<union> as2"
   @end
 @qed
@@ -405,7 +412,7 @@ lemma new_addrs_bind [rewrite]:
   "lim h \<le> lim h' \<Longrightarrow> lim h' \<le> lim h'' \<Longrightarrow> new_addrs h' (new_addrs h as h') h'' = new_addrs h as h''" by auto2
 
 fun success_run :: "'a Heap \<Rightarrow> pheap \<Rightarrow> pheap \<Rightarrow> 'a \<Rightarrow> bool" where
-  "success_run f (h, as) (h', as') r \<longleftrightarrow>
+  "success_run f (pHeap h as) (pHeap h' as') r \<longleftrightarrow>
     as' = new_addrs h as h' \<and> run f (Some h) (Some h') r \<and> relH {a. a < lim h \<and> a \<notin> as} h h' \<and> lim h \<le> lim h'"
 setup {* add_rewrite_rule @{thm success_run.simps} *}
 
@@ -413,43 +420,42 @@ lemma success_run_bind:
   "success_run f h h' r \<Longrightarrow> success_run (g r) h' h'' r' \<Longrightarrow> success_run (f \<bind> g) h h'' r'" by auto2
 
 lemma success_run_next: "success_run f h h'' r' \<Longrightarrow>
-  \<forall>h'. \<sigma> = Some (fst h') \<and> success_run (f \<bind> g) h h' r \<longrightarrow> \<not> h' \<Turnstile> Q \<Longrightarrow>
-  \<forall>h'. \<sigma> = Some (fst h') \<and> success_run (g r') h'' h' r \<longrightarrow> \<not> h' \<Turnstile> Q" by auto2
+  \<forall>h'. \<sigma> = Some (heapOf h') \<and> success_run (f \<bind> g) h h' r \<longrightarrow> \<not> h' \<Turnstile> Q \<Longrightarrow>
+  \<forall>h'. \<sigma> = Some (heapOf h') \<and> success_run (g r') h'' h' r \<longrightarrow> \<not> h' \<Turnstile> Q" by auto2
 
 lemma hoare_triple_def' [rewrite]:
-  "<P> c <Q> \<longleftrightarrow> (\<forall>h \<sigma> r. h \<Turnstile> P \<longrightarrow> run c (Some (fst h)) \<sigma> r \<longrightarrow>
-    (\<sigma> \<noteq> None \<and> (the \<sigma>, new_addrs (fst h) (snd h) (the \<sigma>)) \<Turnstile> Q r \<and>
-     relH {a . a < lim (fst h) \<and> a \<notin> (snd h)} (fst h) (the \<sigma>) \<and>
-     lim (fst h) \<le> lim (the \<sigma>)))" using hoare_triple_def by fastforce
+  "<P> c <Q> \<longleftrightarrow> (\<forall>h \<sigma> r. h \<Turnstile> P \<longrightarrow> run c (Some (heapOf h)) \<sigma> r \<longrightarrow>
+    (\<sigma> \<noteq> None \<and> pHeap (the \<sigma>) (new_addrs (heapOf h) (addrOf h) (the \<sigma>)) \<Turnstile> Q r \<and>
+     relH {a . a < lim (heapOf h) \<and> a \<notin> (addrOf h)} (heapOf h) (the \<sigma>) \<and>
+     lim (heapOf h) \<le> lim (the \<sigma>)))" using hoare_triple_def
+  by (smt Collect_cong pheap.collapse pheap.sel(1) pheap.sel(2))
 
 lemma hoare_tripleE':
-  "<P> c <Q> \<Longrightarrow> h \<Turnstile> P * Ru \<Longrightarrow> run c (Some (fst h)) \<sigma> r \<Longrightarrow>
-   \<exists>h'. h' \<Turnstile> Q r * Ru \<and> \<sigma> = Some (fst h') \<and> success_run c h h' r"
+  "<P> c <Q> \<Longrightarrow> h \<Turnstile> P * Ru \<Longrightarrow> run c (Some (heapOf h)) \<sigma> r \<Longrightarrow>
+   \<exists>h'. h' \<Turnstile> Q r * Ru \<and> \<sigma> = Some (heapOf h') \<and> success_run c h h' r"
 @proof @have "<P * Ru> c <\<lambda>r. Q r * Ru>" @qed
 
 lemma hoare_tripleI:
-  "\<not><P> c <Q> \<Longrightarrow> \<exists>h \<sigma> r. h \<Turnstile> P \<and> run c (Some (fst h)) \<sigma> r \<and>
-   (\<forall>h'. \<sigma> = Some (fst h') \<and> success_run c h h' r \<longrightarrow> \<not>h' \<Turnstile> Q r)" by auto2
+  "\<not><P> c <Q> \<Longrightarrow> \<exists>h \<sigma> r. h \<Turnstile> P \<and> run c (Some (heapOf h)) \<sigma> r \<and>
+   (\<forall>h'. \<sigma> = Some (heapOf h') \<and> success_run c h h' r \<longrightarrow> \<not>h' \<Turnstile> Q r)" by auto2
 
 lemma hoare_triple_mp:
   "<P> c <Q> \<Longrightarrow> h \<Turnstile> P * Ru \<Longrightarrow> success_run c h h' r \<Longrightarrow> h' \<Turnstile> (Q r) * Ru"
 @proof @have "<P * Ru> c <\<lambda>r. Q r * Ru>" @qed
 
 lemma hoare_tripleE'':
-  "<P> c <Q> \<Longrightarrow> h \<Turnstile> P * Ru \<Longrightarrow> run (c \<bind> g) (Some (fst h)) \<sigma> r \<Longrightarrow>
-   \<exists>r' h'. run (g r') (Some (fst h')) \<sigma> r \<and> h' \<Turnstile> Q r' * Ru \<and> success_run c h h' r'"
+  "<P> c <Q> \<Longrightarrow> h \<Turnstile> P * Ru \<Longrightarrow> run (c \<bind> g) (Some (heapOf h)) \<sigma> r \<Longrightarrow>
+   \<exists>r' h'. run (g r') (Some (heapOf h')) \<sigma> r \<and> h' \<Turnstile> Q r' * Ru \<and> success_run c h h' r'"
 @proof
   @have "<P * Ru> c <\<lambda>r. Q r * Ru>" @then
-  @obtain \<sigma>' r' where "run c (Some (fst h)) \<sigma>' r'"
+  @obtain \<sigma>' r' where "run c (Some (heapOf h)) \<sigma>' r'"
 @qed
-
-lemma effect_bind [forward]:
-  "effect (f \<bind> g) h h'' r' \<Longrightarrow> \<exists>h' r. effect f h h' r \<and> effect (g r) h' h'' r'"
-  by (elim effect_elims) auto
 
 setup {* del_prfstep_thm @{thm success_run.simps} *}
 setup {* del_prfstep_thm @{thm hoare_triple_def} *}
 setup {* del_prfstep_thm @{thm hoare_triple_def'} *}
+setup {* fold del_prfstep_thm [@{thm pheap.collapse}, @{thm pheap.simps(1)}] *}
+setup {* fold del_prfstep_thm @{thms pheap.sel} *}
 
 subsection {* Definition of procedures *}
 
